Partial work on implementing partial reduction

src/Experiments/SimplyTypedArithmetic.v
@@ -360,6 +360,590 @@ Module Compilers.
 
   Definition Interp {t} (e : Expr t) := interp (e _).
 
+  Definition const {var t} (v : type.interp t) : @expr var t
+    := Op (op.Const v) TT.
+
+  Section option_partition.
+    Context {A : Type} (f : A -> option Datatypes.bool).
+    Fixpoint option_partition (l : list A) : option (list A * list A)
+      := match l with
+         | nil => Some (nil, nil)
+         | cons x tl
+           => match option_partition tl, f x with
+              | Some (g, d), Some fx
+                => Some (if fx then (x :: g, d) else (g, x :: d))
+              | _, _ => None
+              end
+         end.
+  End option_partition.
+  Section option_flat_map.
+    Context {A B : Type} (f : A -> option (list B)).
+    Fixpoint option_flat_map (l : list A) : option (list B)
+      := match l with
+         | nil => Some nil
+         | cons x t => match f x, option_flat_map t with
+                       | Some fx, Some ft
+                         => Some (fx ++ ft)
+                       | _, _ => None
+                       end
+         end.
+  End option_flat_map.
+
+  Definition lift_option_list {A} (ls : list (option A)) : option (list A)
+    := list_rect
+         (fun _ => _)
+         (Some nil)
+         (fun x _ xs
+          => match x, xs with
+             | Some x, Some xs => Some (cons x xs)
+             | _, _ => None
+             end)
+         ls.
+
+  Section invert.
+    Context {var : type -> Type}.
+
+    Definition invert_Var {t} (e : @expr var t) : option (var t)
+      := match e with
+         | Var t v => Some v
+         | _ => None
+         end.
+
+    Definition invert_Abs {s d} (e : @expr var (type.arrow s d)) : option (var s -> @expr var d)
+      := match e in expr t return option match t with
+                                         | type.arrow _ _ => _
+                                         | _ => True
+                                         end with
+         | Abs s d f => Some f
+         | _ => None
+         end.
+
+    Definition invert_Pair {A B} (e : @expr var (type.prod A B)) : option (@expr var A * @expr var B)
+      := match e in expr t return option match t with
+                                         | type.prod _ _ => _
+                                         | _ => True
+                                         end with
+         | Pair _ _ a b => Some (a, b)
+         | _ => None
+         end.
+
+    Definition invert_Op {t} (e : @expr var t) : option { s : _ & op s t * @expr var s }%type
+      := match e with
+         | Op s d opc args => Some (existT _ s (opc, args))
+         | _ => None
+         end.
+
+    Definition invert_OpConst {t} (e : @expr var t) : option (type.interp t)
+      := match invert_Op e with
+         | Some (existT s (opc, args))
+           => match opc with
+              | op.Const t v => Some v
+              | _ => None
+              end
+         | None => None
+         end.
+
+    Definition invert_op_S (e : @expr var type.nat) : option (@expr var type.nat)
+      := match invert_Op e with
+         | Some (existT s (opc, args))
+           => match opc in op s d return expr s -> option (expr type.nat) with
+              | op.S => fun args => Some args
+              | _ => fun _ => None
+              end args
+         | None => None
+         end.
+
+    Definition invert_Z (e : @expr var type.Z) : option Z := invert_OpConst e.
+    Definition invert_bool (e : @expr var type.bool) : option bool := invert_OpConst e.
+    Fixpoint invert_nat_full (e : @expr var type.nat) : option nat
+      := match e with
+         | Op _ _ op.S args
+           => option_map S (invert_nat_full args)
+         | Op _ _ (op.Const type.nat v) _
+           => Some v
+         | _ => None
+         end.
+    (* oh, the horrors of not being able to use non-linear deep pattern matches *)
+    Fixpoint invert_list_full {t} (e : @expr var (type.list t))
+      : option (list (@expr var t))
+      := match e in expr t return option match t with
+                                         | type.list t => list (expr t)
+                                         | _ => True
+                                         end
+         with
+         | Op s d opc args
+           => match opc in op s d
+                    return option match s with
+                                  | type.prod A (type.list B) => expr A * list (expr B)
+                                  | _ => True
+                                  end
+                           -> option match d with
+                                     | type.list t => list (expr t)
+                                     | _ => True
+                                     end
+              with
+              | op.Const (type.list _) v => fun _ => Some (List.map const v)
+              | op.cons _ => option_map (fun '(x, xs) => cons x xs)
+              | op.nil _ => fun _ => Some nil
+              | _ => fun _ => None
+              end
+                (match args in expr t
+                       return option match t with
+                                     | type.prod A (type.list B) => expr A * list (expr B)
+                                     | _ => True
+                                     end
+                 with
+                 | Pair _ (type.list _) x xs
+                   => match @invert_list_full _ xs with
+                      | Some xs => Some (x, xs)
+                      | None => None
+                      end
+                 | _ => None
+                 end)
+         | _ => None
+         end.
+    (*Section with_map.
+      (* oh, the horrors of not being able to use non-linear deep
+         pattern matches.  Luckily Coq's guard checker unfolds things,
+         so as long as the thing we need to evaluate at the bottom is
+         generic in what type it's looking at, we're good.  We can
+         even give it data of the right type, which we need, but it
+         costs us a lot *)
+      Context (extra_dataT : type -> Type) {U} (f : forall t (d : extra_dataT t), @expr var t -> U t d).
+      Local Notation list_to_extra_dataT t
+        := (match t%ctype return Type with
+            | type.list t' => extra_dataT t'
+            | _ => True
+            end).
+      Local Notation list_to_forall_data_option_list t
+        := (forall (d : list_to_extra_dataT t),
+               option (match t%ctype as t'
+                             return list_to_extra_dataT t' -> Type
+                       with
+                       | type.list t' => fun d => list (U t' d)
+                       | _ => fun _ => True
+                       end d)).
+      Local Notation prod_list_to_extra_dataT t
+        := (match t%ctype return Type with
+            | type.prod _ (type.list t') => extra_dataT t'
+            | _ => True
+            end).
+      Local Notation prod_list_to_forall_data_option_list t
+        := (forall (d : prod_list_to_extra_dataT t),
+               option (match t%ctype as t'
+                             return prod_list_to_extra_dataT t' -> Type
+                       with
+                       | type.prod A (type.list t') => fun d => (expr A * list (U t' d))%type
+                       | _ => fun _ => True
+                       end d)).
+
+
+
+      Fixpoint invert_map_list_full {t} (e : @expr var (type.list t))
+        : forall d : extra_dataT t, option (list (U t d))
+      := match e in expr t return list_to_forall_data_option_list t
+           with
+           | Op s d opc args
+             => match opc in op s d
+                      return (prod_list_to_forall_data_option_list s
+                              -> list_to_forall_data_option_list d)
+                with
+                | op.Const (type.list _) v
+                  => fun _ data => Some (List.map (f _ data) (List.map const v))
+                | op.cons _
+                  => fun xs data
+                     => option_map (fun '(x, xs) => cons (f _ data x) xs) (xs data)
+                | op.nil _
+                  => fun _ _ => Some nil
+                | _ => fun _ _ => None
+                end
+                  (match args in expr t
+                         return prod_list_to_forall_data_option_list t
+                   with
+                   | Pair _ (type.list _) x xs
+                     => fun data
+                        => match @invert_map_list_full _ xs data with
+                           | Some xs => Some (x, xs)
+                           | None => None
+                           end
+                   | _ => fun _ => None
+                   end)
+           | _ => fun _ => None
+           end.
+    End with_map.*)
+  End invert.
+
+  Section gallina_reify.
+    Context {var : type -> Type}.
+    Definition reify_list {t} (ls : list (@expr var t)) : @expr var (type.list t)
+      := list_rect
+           (fun _ => _)
+           (Op op.nil TT)
+           (fun x _ xs => Op op.cons (x, xs))
+           ls.
+  End gallina_reify.
+
+
+  Module arguments.
+    Inductive arguments : type -> Set :=
+    | generic {T} : arguments T
+    (*| cps {T} (aT : arguments T) : arguments T*)
+    | arrow {A B} (aB : arguments B) : arguments (A -> B)
+    | unit : arguments type.unit
+    | prod {A B} (aA : arguments A) (aB : arguments B) : arguments (A * B)
+    | list {T} (aT : arguments T) : arguments (type.list T)
+    | nat : arguments type.nat
+    | Z : arguments type.Z
+    | bool : arguments type.bool.
+
+    Fixpoint ground {t : type} : arguments t
+      := match t with
+         | type.unit => unit
+         | type.prod A B => prod (@ground A) (@ground B)
+         | type.arrow s d => arrow (@ground d)
+         | type.list A => list (@ground A)
+         | type.nat => nat
+         | type.Z => Z
+         | type.bool => bool
+         end.
+
+    Module type.
+      Local Notation interp_type := type.interp.
+      Section interp.
+        Context (var_dom var_cod : type -> Type).
+        Fixpoint interp {t} (a : arguments t) : Type
+          := match a with
+             | generic T => var_cod T
+             (*| cps T aT => forall U, (@interp T aT -> var U) -> var U*)
+             | arrow A B aB => var_dom A -> @interp B aB
+             | unit => Datatypes.unit
+             | prod A B aA aB => @interp A aA * @interp B aB
+             | list T aT => Datatypes.list (@interp T aT)
+             | nat => Datatypes.nat
+             | Z => BinInt.Z
+             | bool => Datatypes.bool
+             end%type.
+      End interp.
+
+      Section ground.
+        Context {var_dom var_cod : type -> Type}.
+        Fixpoint const_of_ground {t}
+          : interp_type t -> option (interp var_dom (@expr var_cod) (@ground t))
+          := match t return interp_type t -> option (interp var_dom expr (@ground t)) with
+             | type.prod A B
+               => fun '((a, b) : interp_type A * interp_type B)
+                  => match @const_of_ground A a, @const_of_ground B b with
+                     | Some a', Some b' => Some (a', b')
+                     | _, _ => None
+                     end
+             | type.arrow s d => fun _ => None
+             | type.list A
+               => fun ls : Datatypes.list (interp_type A)
+                  => lift_option_list
+                       (List.map (@const_of_ground A) ls)
+             | type.unit
+             | type.nat
+             | type.Z
+             | type.bool
+               => fun v => Some v
+             end.
+      End ground.
+
+      Module option.
+        Section interp.
+          Context (var_dom var_cod : type -> Type).
+          Fixpoint interp {t} (a : arguments t) : Type
+            := match a with
+               | generic T => var_cod T
+               (*| cps T aT => forall U, (@interp T aT -> var U) -> var U*)
+               | arrow A B aB => var_dom A -> @interp B aB
+               | unit => Datatypes.unit
+               | prod A B aA aB => option (@interp A aA * @interp B aB)
+               | list T aT => option (Datatypes.list (@interp T aT))
+               | nat => option Datatypes.nat
+               | Z => option BinInt.Z
+               | bool => option Datatypes.bool
+               end%type.
+        End interp.
+
+        Section flat_interp.
+          Context (var_generic var_dom : type -> Type) (var_cod : forall t, arguments t -> Type).
+          Fixpoint flat_interp {t} (a : arguments t) : Type
+            := match a with
+               | generic T => var_generic T
+               (*| cps T aT => forall U, (@interp T aT -> var U) -> var U*)
+               | arrow A B aB => var_dom A -> var_cod B aB
+               | unit => Datatypes.unit
+               | prod A B aA aB => @flat_interp A aA * @flat_interp B aB
+               | list T aT => Datatypes.list (@flat_interp T aT)
+               | nat => Datatypes.nat
+               | Z => BinInt.Z
+               | bool => Datatypes.bool
+               end%type.
+        End flat_interp.
+
+        Definition interp_to_arrow_or_generic var_dom var_cod {t} a
+          := @flat_interp var_cod var_dom (@interp var_dom var_cod) t a.
+
+        Section lift_option.
+          Context {var_dom var_cod : type -> Type}.
+          Fixpoint lift_interp {t} {a : arguments t}
+            : interp var_dom var_cod a -> option (interp_to_arrow_or_generic var_dom var_cod a)
+            := match a in arguments t
+                     return interp var_dom var_cod a -> option (interp_to_arrow_or_generic var_dom var_cod a)
+               with
+               | prod A B aA aB
+                 => fun ab : option (interp _ _ aA * interp _ _ aB)
+                    => match ab with
+                       | Some (a, b)
+                         => match @lift_interp A aA a, @lift_interp B aB b with
+                            | Some a, Some b => Some (a, b)
+                            | _, _ => None
+                            end
+                       | None => None
+                       end
+               | list T aT
+                 => fun ls : option (Datatypes.list (interp _ _ aT))
+                    => match ls with
+                       | Some ls
+                         => lift_option_list
+                              (List.map (@lift_interp T aT) ls)
+                       | None => None
+                       end
+               | arrow _ _ _
+               | generic _
+               | unit
+                 => fun v => Some v
+               | nat
+               | Z
+               | bool
+                 => fun x => x
+               end.
+        End lift_option.
+      End option.
+    End type.
+
+    Module expr.
+      Section interp.
+        Context (var : type -> Type).
+        Fixpoint interp {t} (a : arguments t)
+          : @expr var t -> type.option.interp (@expr var) (@expr var) a
+          := match a in arguments t return expr t -> type.option.interp expr expr a with
+             | generic T => fun e => e
+             (*| cps T aT => fun e*)
+             | arrow A B aB
+               => fun e arg
+                  => @interp
+                       B aB
+                       match invert_Abs e, invert_Var arg with
+                       | Some f, Some arg => f arg
+                       | _, _ => Op op.App (e, arg)
+                       end
+             | unit => fun _ => tt
+             | prod A B aA aB
+               => fun e
+                  => option_map (fun '(a, b)
+                                 => (@interp A aA a, @interp B aB b))
+                                (invert_Pair e)
+             | list T aT
+               => fun e
+                  => option_map
+                       (List.map (@interp T aT))
+                       (invert_list_full e)
+             | nat => invert_nat_full
+             | Z => invert_Z
+             | bool => invert_bool
+             end.
+      End interp.
+
+      Section reify.
+        Context (var : type -> Type).
+        Fixpoint reify {t} (a : arguments t)
+          : type.interp var (@expr var) a -> @expr var t
+          := match a in arguments t return type.interp var expr a -> expr t with
+             | generic T => fun e => e
+             | arrow A B aB => fun f => Abs (fun x => @reify B aB (f x))
+             | unit => fun _ => TT
+             | prod A B aA aB
+               => fun '((a, b) : type.interp _ _ aA * type.interp _ _ aB)
+                  => (@reify A aA a, @reify B aB b)%expr
+             | list T aT
+               => fun ls
+                  => reify_list (List.map (@reify T aT) ls)
+             | nat => @const var type.nat
+             | Z => @const var type.Z
+             | bool => @const var type.bool
+             end.
+      End reify.
+    End expr.
+
+    Module Export Notations.
+      Delimit Scope arguments_scope with arguments.
+      Bind Scope arguments_scope with arguments.
+      Notation "()" := unit : arguments_scope.
+      Notation "A * B" := (prod A B) : arguments_scope.
+      Notation "A -> B" := (@arrow A _ B) (only printing) : arguments_scope.
+      Notation "A -> B" := (arrow B) (only parsing) : arguments_scope.
+      Global Coercion generic : type.type >-> arguments.
+      Notation arguments := arguments.
+    End Notations.
+
+    Module op.
+      Local Open Scope arguments_scope.
+      Definition lookup {s d} (opc : op s d) : arguments s * arguments d
+        := match opc in op s d return arguments s * arguments d with
+           | op.Const t v => (generic, ground)
+           | op.Let_In tx tC => (tx * (tx -> tC), generic)
+           | op.App s d => ((s -> d) * s, generic)
+           | op.S => (ground, ground)
+           | op.nil t => (generic, ground)
+           | op.cons t => (t * list t, list t)
+           | op.fst A B => (A * B, generic)
+           | op.snd A B => (A * B, generic)
+           | op.bool_rect T => (T * T * bool, generic)
+           | op.nat_rect P => (P * (nat -> P -> P) * nat, generic)
+           | op.pred => (nat, ground)
+           | op.List_seq => (nat * nat, ground)
+           | op.List_repeat A => (A * nat, list A)
+           | op.List_combine A B => (list A * list B, list (A * B))
+           | op.List_map A B => ((A -> B) * list A, list B)
+           | op.List_flat_map A B => ((A -> list B) * list A, list B)
+           | op.List_partition A => ((A -> bool) * list A, list A * list A)
+           | op.List_app A => (list A * list A, list A)
+           | op.List_fold_right A B => ((B -> A -> A) * A * list B, generic)
+           | op.List_update_nth T => (nat * (T -> T) * list T, list T)
+           | op.Z_runtime_mul => (Z * Z, Z)
+           | op.Z_runtime_add => (Z * Z, Z)
+           | op.Z_add => (Z * Z, Z)
+           | op.Z_mul => (Z * Z, Z)
+           | op.Z_pow => (Z * Z, Z)
+           | op.Z_opp => (Z, Z)
+           | op.Z_div => (Z * Z, Z)
+           | op.Z_modulo => (Z * Z, Z)
+           | op.Z_eqb => (Z * Z, bool)
+           | op.Z_of_nat => (nat, Z)
+           end.
+
+      Definition lookup_src {s d} opc := fst (@lookup s d opc).
+      Definition lookup_dst {s d} opc := snd (@lookup s d opc).
+
+      Definition option_map_prod {A B C} (f : A -> B -> C) (v : option (option A * option B))
+        : option C
+        := match v with
+           | Some (Some a, Some b) => Some (f a b)
+           | _ => None
+           end.
+
+
+
+      Definition rewrite
+                 {var : type -> Type}
+                 {s d} (opc : op s d)
+                 (exploded_arguments : type.option.interp (@expr var) (@expr var) (lookup_src opc))
+        : option (type.interp var (@expr var) (lookup_dst opc))
+        := match opc in op s d
+                 return
+                 (forall (exploded_arguments' : option (type.option.interp_to_arrow_or_generic expr expr (lookup_src opc))),
+                     option (type.interp var expr (lookup_dst opc)))
+           with
+           | op.Const t v => fun _ => arguments.type.const_of_ground v
+           | op.Let_In tx tC
+             => option_map
+                  (fun '(ex, eC)
+                   => match invert_Var ex, invert_OpConst ex with
+                      | Some v, _ => eC ex
+                      | None, Some v => eC ex
+                      | None, None => Op op.Let_In (ex, Abs (fun v => eC (Var v)))
+                      end)
+           | op.App s d => option_map (fun '(f, x) => f x)
+           | op.S as opc
+           | op.pred as opc
+           | op.Z_runtime_mul as opc
+           | op.Z_runtime_add as opc
+           | op.Z_add as opc
+           | op.Z_mul as opc
+           | op.Z_pow as opc
+           | op.Z_opp as opc
+           | op.Z_div as opc
+           | op.Z_modulo as opc
+           | op.Z_eqb as opc
+           | op.Z_of_nat as opc
+             => option_map (op.interp opc)
+           | op.nil t => fun _ => Some (@nil (type.interp _ _ ground))
+           | op.cons t => option_map (op.curry2 cons)
+           | op.fst A B => option_map (@fst (expr A) (expr B))
+           | op.snd A B => option_map (@snd (expr A) (expr B))
+           | op.bool_rect T => option_map (op.curry3 (bool_rect (fun _ => _)))
+           | op.nat_rect P
+             => option_map
+                  (fun '(O_case, S_case, v)
+                   => nat_rect (fun _ => expr P) O_case (fun n (v : expr P) => S_case (@const _ type.nat n) v) v)
+           | op.List_seq => option_map (op.curry2 List.seq)
+           | op.List_repeat A => option_map (op.curry2 (@List.repeat (expr A)))
+           | op.List_combine A B => option_map (op.curry2 (@List.combine (expr A) (expr B)))
+           | op.List_map A B => option_map (op.curry2 (@List.map (expr A) (expr B)))
+           | op.List_flat_map A B
+             => fun args : option ((expr A -> option (Datatypes.list (expr B))) * Datatypes.list (expr A))
+                => match args with
+                   | Some (f, ls) => option_flat_map f ls
+                   | None => None
+                   end
+           | op.List_partition A
+             => fun args : option ((expr A -> option Datatypes.bool) * Datatypes.list (expr A))
+                => match args with
+                   | Some (f, ls) => option_partition f ls
+                   | None => None
+                   end
+           | op.List_app A => option_map (op.curry2 (@List.app (expr A)))
+           | op.List_fold_right A B => option_map (op.curry3 (@List.fold_right (expr A) (expr B)))
+           | op.List_update_nth T => option_map (op.curry3 (@update_nth (expr T)))
+           end
+             (type.option.lift_interp exploded_arguments).
+    End op.
+  End arguments.
+  Export arguments.Notations.
+
+  Section partial_reduce.
+    Context {var : type -> Type}.
+
+    Fixpoint partial_reduce_cps {T} {t} (e : @expr (@expr var) t)
+      : (@expr var t -> @expr var T) -> @expr var T
+      := match e in expr t return (expr t -> expr T) -> expr T with
+         | TT => fun k => k TT
+         | Pair A B a b
+           => fun k
+              => @partial_reduce_cps
+                   T A a
+                   (fun a'
+                    => @partial_reduce_cps
+                         T B b
+                         (fun b' => k (Pair a' b')))
+         | Var t v => fun k => k v
+         | Abs s d f
+           => fun k
+              => k (Abs (fun x => @partial_reduce_cps _ d (f (Var x)) id))
+         | Op s d opc args
+           => fun k
+              => @partial_reduce_cps
+                   T s args
+                   (fun args'
+                    => k
+                         match arguments.op.rewrite
+                                 opc
+                                 (arguments.expr.interp _ _ args')
+                         with
+                         | Some e => arguments.expr.reify _ _ e
+                         | None => Op opc args'
+                         end)
+         end.
+
+    Definition partial_reduce {t} (e : @expr (@expr var) t) : @expr var t
+      := @partial_reduce_cps t t e id.
+  End partial_reduce.
+
+  Definition PartialReduce {t} (e : Expr t) : Expr t
+    := fun var => @partial_reduce var t (e _).
+
   Ltac is_known_const_cps2 term on_success on_failure :=
     let recurse term := is_known_const_cps2 term on_success on_failure in
     lazymatch term with
@@ -658,6 +1242,13 @@ Example base_25_5_mul (*(f0 f1 f2 f3 f4 f5 f6 f7 f8 f9 g0 g1 g2 g3 g4 g5 g6 g7 g
   cbv [n].
   cbv delta [mulmod w to_associational mul to_associational reduce from_associational add_to_nth zeros place split].
   Reify_rhs ().
+  let e := match goal with |- _ = Interp ?e => e end in
+  pose e as E.
+  exfalso.
+  Timeout 2 vm_compute in E.
+  pose (PartialReduce E) as E'.
+  Timeout 2 vm_compute in E'.
+
   (*cbv -[runtime_mul runtime_add]; cbv [runtime_mul runtime_add].
   ring_simplify_subterms.*)
 (* ?fg =
